src/zfc_consistent.lean
@@ -15,13 +15,17 @@ end
 
 local notation `Set'` := L_ZFC_structure_of_Set
 
-instance  has_mem_Set'_Set' : (has_mem Set' Set') := ⟨Set.mem⟩
+instance has_mem_Set'_Set' : (has_mem Set' Set') := ⟨Set.mem⟩
 
 instance has_mem_Set_Set' : has_mem Set.{0} Set' := ⟨Set.mem⟩
 
 instance has_emptyc_Set' : has_emptyc Set' := ⟨Set.empty⟩
 
 lemma  empty_subset : ∀ x: Set',  Set.empty ⊆ x := by tidy 
+
+lemma Set'_Set : ↥Set' = Set := by refl
+
+@[simp]lemma Set'_Set_2 {p : (by exact ↥Set') → Prop} : (λ x, p x) = λ x : Set, p x := by refl
 
 lemma Set'_has_mem : has_mem ↥Set' ↥Set' := ⟨ Set.mem ⟩
 local notation h :: t  := dvector.cons h t
@@ -54,10 +58,16 @@ begin
 end
 set_option trace.app_builder true
 
-@[simp]lemma Set'_realize_empty : @realize_bounded_formula L_ZFC Set' 1 0 (Set.empty :: dvector.nil) is_emptyset dvector.nil :=
+@[simp]lemma Set'_realize_is_empty : ∀ x, (@realize_bounded_formula L_ZFC Set' _ _ ([x]) is_emptyset dvector.nil ↔ x = ∅) :=
 begin
-rw is_emptyset, simp, intros, change x ∉ ∅, intros a, induction x, work_on_goal 0 {cases a, cases a_w, cases a_w}, refl
+  intro x, unfold is_emptyset,
+   simp only [not_exists, fol.realize_bounded_formula_ex, Set'_mem_mem,
+   fol.realize_bounded_formula, fol.realize_bounded_formula_not, fol.realize_bounded_term],
+   symmetry, apply Set.eq_empty
 end
+
+@[simp]lemma Set'_realize_empty : @realize_bounded_formula L_ZFC Set' 1 0 (Set.empty :: dvector.nil) is_emptyset dvector.nil :=
+by rw[Set'_realize_is_empty]; refl
 
 -- set_option trace.simplify.rewrite true
 
@@ -76,8 +86,6 @@ begin
   refine ⟨⋃ x, _⟩, intro z, rw[@Set.mem_Union x z], finish
 end
 
-
-
 lemma Set'_models_powerset : axiom_of_powerset ∈ Th Set' := 
 begin
   simp only [Th, axiom_of_powerset, small,  fol.realize_bounded_formula_ex,
@@ -92,16 +100,46 @@ lemma Set'_models_choice : axiom_of_choice ∈ Th Set' := sorry
 
 lemma Set'_models_infinity : axiom_of_infinity ∈ Th Set' :=
 begin
-simp [has_mem.mem, set.mem, Th, set_of, axiom_of_infinity,satisfied_in], 
-refine ⟨Set.omega, _⟩,
-refine ⟨_,_⟩,
-refine ⟨Set.empty,_⟩,
-refine ⟨Set'_realize_empty, by {change Set.empty ∈ Set.omega, exact Set.omega_zero}⟩,
-intros, refine ⟨Set.insert x x, _⟩,
-refine ⟨_,@Set.omega_succ x a⟩,
-change x ∈ Set.insert x x,
-exact (iff.mpr Set.mem_insert (or.inl (refl x)))
+  simp [has_mem.mem, set.mem, Th, set_of, axiom_of_infinity,satisfied_in], 
+  refine ⟨Set.omega, _⟩, refine ⟨_,_⟩, refine ⟨Set.empty,_⟩,
+  refine ⟨Set'_realize_empty, by {change Set.empty ∈ Set.omega, exact Set.omega_zero}⟩,
+  intros, refine ⟨Set.insert x x, _⟩, refine ⟨_,@Set.omega_succ x a⟩,
+  exact (iff.mpr Set.mem_insert (or.inl (refl x)))
 end
+
+lemma Set'_models_infinity' : axiom_of_infinity' ∈ Th Set' :=
+begin
+  simp [has_mem.mem, set.mem, Th, set_of, axiom_of_infinity' ,satisfied_in,realize_cast_bounded_formula], 
+  refine ⟨Set.omega, _⟩, intro x, refine ⟨_,_⟩,
+  {intro H_x, change Set.mem x _, change _ ∈ Set.omega,
+  suffices : x = Set.empty, by rw[this]; apply Set.omega_zero, exact H_x},
+  intro y, conv in (dvector.nth _ _ _) {change x}, conv in (dvector.nth _ _ _) {change y},
+  change Set.mem y Set.omega → _, intro H,
+  exact ⟨Set.insert y y, ⟨iff.mpr Set.mem_insert (or.inl (by refl)), @Set.omega_succ y H⟩⟩
+end
+
+lemma Set'_models_shallow_infinity : Set_axiom_of_infinity :=
+begin
+  unfold Set_axiom_of_infinity Set_is_emptyset, refine ⟨Set.omega, _⟩,
+  split,
+    {refine ⟨∅, ⟨_, Set.omega_zero⟩⟩, apply Set.mem_empty},
+    {intros z H, refine ⟨Set.insert z z, ⟨iff.mpr Set.mem_insert (or.inl (by refl)), @Set.omega_succ z H⟩⟩},
+end
+
+lemma shallow_infinity_iff_shallow_infinity' : Set_axiom_of_infinity ↔ Set_axiom_of_infinity' :=
+  sorry
+
+lemma Set'_infinity_shallow_infinity : Set'[axiom_of_infinity] ↔ Set_axiom_of_infinity  :=
+  sorry
+
+lemma Set'_infinity'_shallow_infinity' :  Set'[axiom_of_infinity'] ↔ Set_axiom_of_infinity' :=
+  sorry
+ 
+example : axiom_of_infinity ∈ Th(Set') :=
+  Set'_infinity_shallow_infinity.mpr Set'_models_shallow_infinity
+
+example : axiom_of_infinity' ∈ Th(Set') :=
+      Set'_infinity'_shallow_infinity'.mpr $ shallow_infinity_iff_shallow_infinity'.mp Set'_models_shallow_infinity
 
 @[simp]lemma Set'_functional_rw : ∀ c : bounded_formula L_ZFC 2, @realize_bounded_formula L_ZFC Set' 0 0 dvector.nil (functional c) dvector.nil = ∀ x : Set, ∃ y : Set, ∀ w, @realize_bounded_formula L_ZFC Set' 3 0  ([w,y,x]) ( (c ↑' 1 # 1) ⇔ &0 ≃ &1)  dvector.nil := 
 begin
